

# Supplement to Feedback-assisted Decentralized Dynamic Spectrum Access

## APPENDIX

### PROOF OF THEOREM 1

Before presenting the proof of Theorem 1, we first introduce the following concentration inequality [1], which provides an upper tail bound for the sum of possibly dependent bounded random variables.

**Theorem 1.** ([1] Theorem 1.8) Suppose that  $X_1, \dots, X_n$  are random variables such that  $0 \leq X_i \leq 1$ . Set  $p = \frac{1}{n} \sum_{i=1}^n E[X_i]$  and fix a real number  $\vartheta$  such that  $np + 1 < \vartheta < n$ . If  $\epsilon_0 > 0$  satisfies  $\vartheta - 1 = np + n\epsilon_0$ , then

$$P\left(\sum_{i=1}^n X_i \geq \vartheta\right) \leq 2 \exp(-nD(p(1 + \epsilon_0)||p)),$$

where  $D(q||p) = q \ln \frac{q}{p} + (1 - q) \ln \frac{1-q}{1-p}$ .

Now we are ready to proceed with the proof of Theorem 1. We start by relating separation to score differences. The event  $p_i^t \neq p_{i'}^t$  occurs if the prototype maximizing  $S_j(\mathcal{H}_i^t)$  differs from that maximizing  $S_j(\mathcal{H}_{i'}^t)$ . Define the score difference:

$$\Delta_k = S_j(\mathcal{H}_i^t) - S_j(\mathcal{H}_{i'}^t) = [D(p_j; \mathcal{H}_i^t) - D(p_j; \mathcal{H}_{i'}^t)]. \quad (1)$$

The event  $p_i^t = p_{i'}^t$  implies that the maximum scores align, i.e.,  $\arg \max_j S_j(\mathcal{H}_i^t) = \arg \max_j S_j(\mathcal{H}_{i'}^t)$ . A sufficient condition for separation is that for some  $j$ ,  $\Delta_j > 0$ , and for another  $k$ ,  $\Delta_k < 0$ . We focus on a prototype  $j$  expected to favor  $\mathcal{H}_i^t$ .

Since  $\mathcal{D}_H(\mathcal{H}_i^t, \mathcal{H}_{i'}^t) \geq \delta$ , the histories differ at some time steps. We select a prototype  $p_j$  for which the expected per-slot score difference satisfies  $\mathbb{E}[d(s, p_j; \mathcal{H}_i^t) - d(s, p_j; \mathcal{H}_{i'}^t)] \geq \frac{\delta}{c}$ , where  $(s, p_j; \mathcal{H}_i^t)$  is defined as  $d(s, p_j; \mathcal{H}_i^t) = w_a \cdot \mathbb{I}\{a_i^{s-1} = a_j\} + w_M \cdot \mathbb{I}\{M^s = M_j\} + w_m \cdot \mathbb{I}\{m_i^s = m_j\}$ . Then define the per-slot score difference as

$$Y_s = d(s, p_j; \mathcal{H}_i^t) - d(s, p_j; \mathcal{H}_{i'}^t), \quad (2)$$

for  $s = t - W, \dots, t - 1$ . Since  $d(s, p_j; \mathcal{H}) \in [0, w_{t-1-s}]$ , we have,  $Y_s \in [-w_{t-1-s}, w_{t-1-s}]$ . Given  $w_{t-1-s} \leq 1$ , it follows that  $Y_s \in [-1, 1]$ . To normalize this difference, let

$$X_s = \frac{1 + Y_s}{2}, \quad (3)$$

so  $X_s \in [0, 1]$ , which is useful for bounding the probability of separation in the next step.

Next, we compute the expectation of  $X_s$ . Let  $\mu_s = \mathbb{E}[Y_s]$ , where the expectation is taken over any randomness in the history components  $(a_i^s, M^{s+1}, m_i^{s+1})$  such as stochastic actions or feedback and potentially the selection of  $p_j$  if it is random. Then,  $\mathbb{E}[X_s] = \mathbb{E}\left[\frac{1+Y_s}{2}\right] = \frac{1+\mu_s}{2}$ .

Set the average expectation across the window as

$$\begin{aligned} p &= \frac{1}{W} \sum_{s=t-W}^{t-1} \mathbb{E}[X_s] = \frac{1}{W} \sum_{s=t-W}^{t-1} \frac{1 + \mu_s}{2} \\ &= \frac{1}{2} + \frac{1}{2W} \sum_{s=t-W}^{t-1} \mu_s. \end{aligned}$$

Let  $\bar{\mu} = \frac{1}{W} \sum_{s=t-W}^{t-1} \mu_s$ . Thus, we have  $p = \frac{1}{2} + \frac{\bar{\mu}}{2}$ . Now, since  $\mu_s = \mathbb{E}[Y_s] = \mathbb{E}[d(s, p_j; \mathcal{H}_i^t) - d(s, p_j; \mathcal{H}_{i'}^t)]$ , and we chose  $p_j$  such that

$$\mathbb{E}[d(s, p_j; \mathcal{H}_i^t) - d(s, p_j; \mathcal{H}_{i'}^t)] \geq \frac{\delta}{c}$$

, it follows that  $\bar{\mu} = \frac{1}{W} \sum_{s=t-W}^{t-1} \mu_s \geq \frac{\delta}{c}$ , assuming the bound holds uniformly across slots (or adjusting  $c$  if the expectation varies). Therefore, we have  $p = \frac{1}{2} + \frac{\bar{\mu}}{2} \geq \frac{1}{2} + \frac{\delta}{2c}$ .

These random variables and their expectations allow us to bound the probability that  $\Delta_j > 0$  in the next step, leveraging the normalized form of  $X_s$ .

To establish a lower bound on  $P(p_i^t \neq p_{i'}^t)$ , consider the event that the score difference  $\Delta_j = S_j(\mathcal{H}_i^t) - S_j(\mathcal{H}_{i'}^t)$  for the chosen prototype  $p_j$  is positive, where  $p_j$  satisfies  $\mathbb{E}[d(s, p_j; \mathcal{H}_i^t) - d(s, p_j; \mathcal{H}_{i'}^t)] \geq \frac{\delta}{c}$ . Since  $p_i^t \neq p_{i'}^t$  occurs if the maximizing prototypes differ, we have

$$P(p_i^t \neq p_{i'}^t) \geq P(\Delta_j > 0). \quad (4)$$

Given  $\Delta_j = \sum_{s=t-W}^{t-1} Y_s$ , and using the normalized variables  $X_s = \frac{1+Y_s}{2}$ , we express the sum as:

$$\sum_{s=t-W}^{t-1} X_s = \frac{W + \sum_{s=t-W}^{t-1} Y_s}{2},$$

so that  $\Delta_j > 0$  (i.e.,  $\sum_{s=t-W}^{t-1} Y_s > 0$ ) holds if and only if  $\sum_{s=t-W}^{t-1} X_s > \frac{W}{2}$ . Since  $E\left[\sum_{s=t-W}^{t-1} X_s\right] = Wp$ , where  $p = \frac{1}{2} + \frac{\bar{\mu}}{2} \geq \frac{1}{2} + \frac{\delta}{2c}$ , we have  $Wp \geq W\left(\frac{1}{2} + \frac{\delta}{2c}\right) > \frac{W}{2}$ , indicating that  $\sum_{s=t-W}^{t-1} X_s > \frac{W}{2}$  occurs when the sum exceeds its mean. To bound this probability, define a threshold  $\vartheta = Wp + \lambda W \frac{\delta}{c}$ , where  $\lambda > 0$  is a constant to be determined, ensuring  $\vartheta > Wp$ . We require  $Wp + 1 < \vartheta < W$ , which enable the application of Theorem 1 to bound the complementary event  $P\left(\sum_{s=t-W}^{t-1} X_s \leq \frac{W}{2}\right)$ , corresponding to  $\Delta_j \leq 0$ .

The lower bound  $Wp + 1 < \vartheta$  simplifies to  $Wp + 1 < Wp + \lambda W \frac{\delta}{c}$ , which leads to the condition  $\lambda > \frac{c}{W\delta}$ , while the upper bound  $\vartheta < W$  gives  $Wp + \lambda W \frac{\delta}{c} < W$ , which in turn implies  $p + \lambda \frac{\delta}{c} < 1$ .

Since  $p \geq \frac{1}{2} + \frac{\delta}{2c}$ , we deduce that  $1 - p \leq \frac{1}{2} - \frac{\delta}{2c}$ , and hence the condition  $\lambda \frac{\delta}{c} < \frac{1}{2} - \frac{\delta}{2c}$  must hold, which yields  $\lambda < \frac{c}{2\delta} - \frac{1}{2} < \frac{c}{2\delta}$ . Then, for  $W > 2$ , consistent with the window size assumption, we obtain the range  $\frac{c}{W\delta} < \lambda < \frac{c}{2\delta}$ .

Next, define  $\epsilon_0$  such that  $\vartheta - 1 = Wp(1 + \epsilon_0)$ . By equating both expressions for  $\vartheta$ , we obtain  $Wp + \lambda W \frac{\delta}{c} - 1 = Wp(1 + \epsilon_0)$ , which gives  $\epsilon_0 = \frac{\lambda \frac{\delta}{c} - \frac{1}{W}}{p}$ . Furthermore, we observe that  $\epsilon_0 \geq 2\lambda \frac{\delta}{c}$ .

Now apply Theorem 1 to bound the upper tail probability  $P\left(\sum_{s=t-W}^{t-1} X_s \geq \vartheta\right)$ , which requires the KL divergence  $D(p(1 + \epsilon_0)||p)$ . For small  $\epsilon_0$ , the divergence can be approximated as  $D(p(1 + \epsilon_0)||p) \geq \frac{p\epsilon_0^2}{2(1-p)}$ . Substituting  $p \geq \frac{1}{2}$  and  $\epsilon_0 \geq 2\lambda \frac{\delta}{c}$ , we get

$$D(p(1 + \epsilon_0)||p) \geq 2\lambda^2 \left(\frac{\delta}{c}\right)^2. \quad (5)$$

Thus, Theorem 1 yields,  $P\left(\sum_{s=t-W}^{t-1} X_s \geq \vartheta\right) \leq 2 \exp\left(-W \cdot 2\lambda^2 \left(\frac{\delta}{c}\right)^2\right)$ , implying  $P\left(\sum_{s=t-W}^{t-1} X_s < \vartheta\right) \geq 1 - 2 \exp\left(-W \cdot 2\lambda^2 \left(\frac{\delta}{c}\right)^2\right)$ .

Since  $\vartheta = Wp + \lambda W \frac{\delta}{c} \geq W\left(\frac{1}{2} + \frac{\delta}{2c}\right) + \lambda W \frac{\delta}{c} > \frac{W}{2}$ , the event  $\sum_{s=t-W}^{t-1} X_s < \vartheta$  implies  $\sum_{s=t-W}^{t-1} X_s \leq \frac{W}{2}$ , so:

$$\begin{aligned} P\left(\sum_{s=t-W}^{t-1} X_s \leq \frac{W}{2}\right) &\leq P\left(\sum_{s=t-W}^{t-1} X_s < \vartheta\right) \\ &\leq 2 \exp\left(-W \cdot 2\lambda^2 \left(\frac{\delta}{c}\right)^2\right). \end{aligned} \quad (6)$$

Therefore,  $P(\Delta_j \leq 0) \leq 2 \exp\left(-W \cdot 2\lambda^2 \left(\frac{\delta}{c}\right)^2\right)$ , and from (4) and (6), we can write

$$\begin{aligned} P(p_i^t \neq p_{i'}^t) &\geq 1 - P(\Delta_j \leq 0) \\ &\geq 1 - 2 \exp\left(-W \cdot 2\lambda^2 \left(\frac{\delta}{c}\right)^2\right). \end{aligned}$$

Since  $2e^{-x} \leq e^{-x/2}$  for all  $x \geq 2\log(2)$  and let  $c' = \lambda^2 \frac{1}{c^2}$ , we get

$$P(p_i^t \neq p_{i'}^t) \geq 1 - e^{-c'W\delta^2},$$

where  $\lambda$  satisfies the constraints  $\frac{c}{W\delta} < \lambda < \frac{c}{2\delta}$ . Which complete the proof

The bound on  $P(\Delta_j > 0)$  for a single prototype  $p_j$  expected to favor  $\mathcal{H}_i^t$  provides a lower bound on  $P(p_i^t \neq p_{i'}^t)$ . In reality,  $p_i^t \neq p_{i'}^t$  occurs if the maximizer of  $S_j(\mathcal{H}_i^t)$  differs from that of  $S_j(\mathcal{H}_{i'}^t)$ , which may involve multiple prototypes. However, since  $\mathcal{D}_H \geq \delta$ , there exists at least one prototype where the score difference is significant, and our bound captures this dominant effect. A more precise bound could use a union bound over all prototypes, but this suffices for the desired exponential form.

## PROOF OF THEOREM 2

Before presenting the proof of Theorem 2, we state a preliminary result on the convergence of the empirical Q-values under fixed policy to their true Q-values. To analyze the convergence of Algorithm 1, we define the true action-value function for user  $i$ 's policy  $\pi_i$  as:

$$Q_i^{\pi_i}(s_i^{t_e}, a_i^{t_e}) = \mathbb{E}_{\pi_i, \pi_{-i}} \left[ \sum_{l=t_e}^{T_h} \gamma^{l-t_e} r_i^l \mid s_i^{t_e}, a_i^{t_e} \right],$$

and the joint action-value function for joint policy  $\pi$  as

$$Q_\pi(\mathbf{s}, \mathbf{a}) = \frac{1}{N} \sum_{i=1}^N Q_i^{\pi_i}(s_i, a_i). \quad (7)$$

The empirical action-value function  $\tilde{Q}_i(s_i^{t_e}, a_i^{t_e})$  is the average Q-value estimate over  $E$  episodes, and the empirical joint action-value function is:

$$\tilde{Q}_\pi(\mathbf{s}, \mathbf{a}) = \frac{1}{N} \sum_{i=1}^N \tilde{Q}_i(s_i, a_i).$$

The reward  $r_i^{t_e}$  is bounded by  $r_{i,min}^e = 0$  and  $r_{i,max}^e = \frac{1-\gamma^T}{1-\gamma} \max(1, \phi)$ , based on (7). The joint reward bounds are  $R_{min}^e = 0$ ,  $R_{max}^e = \frac{1-\gamma^T}{1-\gamma} \max(1, \phi)$ .

**Lemma 1.** *Let each user  $i \in \mathcal{N}$  follow policy  $\pi_i^e$  in episode  $e$ , generating a joint trajectory  $\boldsymbol{\tau}^e = \{(\mathbf{s}^{t_e}, \mathbf{a}^{t_e}, \mathbf{r}^{t_e})\}_{t=0}^{T-1}$  with valid actions. For a number of episodes  $E > \frac{(R_{max}^e)^2}{2\epsilon^2} \log\left(\frac{2}{\sigma}\right)$ , the empirical joint action-value function satisfies:*

$$P\left(\left|\tilde{Q}_\pi(\mathbf{s}, \mathbf{a}) - Q_\pi(\mathbf{s}, \mathbf{a})\right| \leq \epsilon\right) \geq 1 - \sigma,$$

with probability parameter  $\sigma = 2 \exp\left(-\frac{2\epsilon^2 E}{(R_{max}^e)^2}\right)$ .

*Proof.* The empirical action-value function  $\tilde{Q}_i(s_i^{t_e}, a_i^{t_e})$  for user  $i$  is computed as the average cumulative discounted reward over  $E$  episodes, where each episode  $e$  yields rewards  $r_i^{t_e} \in [0, \max(1, \phi)]$ . The cumulative reward per episode is bounded by:

$$r_{i,min}^e = 0, \quad r_{i,max}^e = \frac{1-\gamma^T}{1-\gamma} \max(1, \phi).$$

Assuming independent trajectories across episodes (due to the stationary environment and fixed policies  $\pi_i^e$  within each episode), we apply the Chernoff-Hoeffding bound to the empirical estimate  $\tilde{Q}_i(s_i^{t_e}, a_i^{t_e})$ :

$$P\left(\left|\tilde{Q}_i(s_i^{t_e}, a_i^{t_e}) - Q_i^{\pi_i}(s_i^{t_e}, a_i^{t_e})\right| \geq \epsilon\right) \leq \exp\left(-\frac{2\epsilon^2 E}{(r_{i,max}^e - r_{i,min}^e)^2}\right). \quad (8)$$

Thus:

$$P\left(\left|\tilde{Q}_i(s_i^{t_e}, a_i^{t_e}) - Q_i^{\pi_i}(s_i^{t_e}, a_i^{t_e})\right| < \epsilon\right) > 1 - \sigma_i,$$

where  $\sigma_i = 2 \exp\left(-\frac{2\epsilon^2 E}{(r_{i,max}^e)^2}\right)$ , since  $r_{i,min}^e = 0$ .

For the joint action-value function, since  $\tilde{Q}_\pi(\mathbf{s}, \mathbf{a}) = \frac{1}{N} \sum_{i=1}^N \tilde{Q}_i(s_i, a_i)$ , the error is:

$$\begin{aligned} \left| \tilde{Q}_\pi(\mathbf{s}, \mathbf{a}) - Q_\pi(\mathbf{s}, \mathbf{a}) \right| &= \frac{1}{N} \left| \sum_{i=1}^N \left( \tilde{Q}_i(s_i, a_i) - Q_i^{\pi_i}(s_i, a_i) \right) \right| \\ &\leq \frac{1}{N} \sum_{i=1}^N \left| \tilde{Q}_i(s_i, a_i) - Q_i^{\pi_i}(s_i, a_i) \right|. \end{aligned} \quad (9)$$

Assuming the same  $\epsilon$  for all users, if  $\left| \tilde{Q}_i(s_i, a_i) - Q_i^{\pi_i}(s_i, a_i) \right| \leq \epsilon$  for each  $i$ , then:

$$\left| \tilde{Q}_\pi(\mathbf{s}, \mathbf{a}) - Q_\pi(\mathbf{s}, \mathbf{a}) \right| \leq \epsilon.$$

The joint error probability is bounded using the union bound and the fact that  $r_{i,max}^e = R_{max}^e$ :

$$P \left( \left| \tilde{Q}_\pi(\mathbf{s}, \mathbf{a}) - Q_\pi(\mathbf{s}, \mathbf{a}) \right| \geq \epsilon \right) \leq 2 \exp \left( -\frac{2\epsilon^2 E}{(R_{max}^e)^2} \right). \quad (10)$$

To ensure the error is at most  $\epsilon$  with probability at least  $1 - \sigma$ , set:

$$2 \exp \left( -\frac{2\epsilon^2 E}{(R_{max}^e)^2} \right) \leq \sigma.$$

Solving for  $E$ :

$$E \geq \frac{(R_{max}^e)^2}{2\epsilon^2} \log \left( \frac{2}{\sigma} \right).$$

Thus, for  $E > \frac{(R_{max}^e)^2}{2\epsilon^2} \log \left( \frac{2}{\sigma} \right)$ , we have:

$$P \left( \left| \tilde{Q}_\pi(\mathbf{s}, \mathbf{a}) - Q_\pi(\mathbf{s}, \mathbf{a}) \right| \leq \epsilon \right) \geq 1 - \sigma,$$

with  $\sigma = 2 \exp \left( -\frac{2\epsilon^2 E}{(R_{max}^e)^2} \right)$ . □

We also state the following theorem on the almost sure convergence of sequences of random variables [2].

**Theorem 2.** ([2] Theorem 1, p. 253) *Let  $\{\xi_n\}_{n \geq 1}$  be a sequence of random variables, and let  $\xi$  be a random variable. Then,  $\xi_n \rightarrow \xi$  almost surely (P.a.s.) if and only if*

$$\lim_{n \rightarrow \infty} \Pr \left( \sup_{k \geq n} |\xi_k - \xi| \geq \varepsilon \right) = 0.$$

for every  $\varepsilon > 0$ .

Now, we proceed with the proof of Theorem 2. From the results of Lemma 1, we establish concentration bounds for the value function in Phase 1 for  $e < ((r_{max}^e - r_{min}^e)/\epsilon)^2 \log(2/\sigma)$ , there exist  $\epsilon > 0$ ,  $\rho > 0$  such that,

$$P \left( \sum_{t=0}^{n^e-1} \gamma^t r_i^{t_e} - \sum_{t=0}^{n^{e-1}-1} \gamma^t r_i^{t_{e-1}} \geq \epsilon \right) \geq \rho, \quad (11)$$

where  $t_e = t + (e-1)T + 1$ ,  $t_{e-1} = t + (e-2)T + 1$ ,  $n^e = |\{t : M^{t_{e-1}} = 1\}|$ , and  $r_i^{t_e}$  is the reward from (7) in Phase 1. Let  $e_\epsilon$  be the first episode for which the monotone nondecreasing sequence  $\sum_{t=0}^{n^e-1} \gamma^t r_i^{t_e}$  becomes strictly larger than  $Q_i^*(s_i^{t_e}, a_i^{t_e}) - \epsilon$ .

$$\begin{aligned} &\text{If } \sum_{t=0}^{n^e-1} \gamma^t r_i^{t_e} \leq Q_i^*(s_i^{t_e}, a_i^{t_e}) - \epsilon, \text{ then} \\ &\mathbb{E} \left[ \sum_{t=0}^{n^e-1} \gamma^t r_i^{t_e} - \sum_{t=0}^{n^{e-1}-1} \gamma^t r_i^{t_{e-1}} \right] \geq \epsilon \rho, \quad \forall e < e_\epsilon. \end{aligned} \quad (12)$$

From this and the fact that  $Q_i^e(s_i^{t_e}, a_i^{t_e})$  is bounded above by  $Q_i^*(s_i^{t_e}, a_i^{t_e})$ ,  $\sum_{t=0}^{n^e-1} \gamma^t r_i^{t_e} - \sum_{t=0}^{n^{e-1}-1} \gamma^t r_i^{t_{e-1}} \geq 0$  when  $n^e \geq n^{e-1}$ , and  $\sum_{t=0}^{n^e-1} \gamma^t r_i^{t_e} \geq 0$  with probability one, we have

$$\begin{aligned}
Q_i^*(s_i^{t_e}, a_i^{t_e}) &\geq \mathbb{E} \left[ \lim_{e \rightarrow \infty} \sum_{t=0}^{n^e-1} \gamma^t r_i^{t_e} \right] = \mathbb{E} \left[ \sum_{t=0}^{n^0-1} \gamma^t r_i^{t_0} \right] + \\
&\quad \mathbb{E} \left[ \sum_{e=0}^{\infty} \left( \sum_{t=0}^{n^{e+1}-1} \gamma^t r_i^{t_{e+1}} - \sum_{t=0}^{n^e-1} \gamma^t r_i^{t_e} \right) \right] \\
&\geq \mathbb{E} \left[ \sum_{t=0}^{n^0-1} \gamma^t r_i^{t_0} \right] + \\
&\quad \mathbb{E} \left[ \sum_{e=0}^{e_\epsilon} \left( \sum_{t=0}^{n^{e+1}-1} \gamma^t r_i^{t_{e+1}} - \sum_{t=0}^{n^e-1} \gamma^t r_i^{t_e} \right) \right] \\
&\geq \mathbb{E} \left[ \sum_{t=0}^{n^0-1} \gamma^t r_i^{t_0} \right] + \epsilon \rho \mathbb{E}[e_\epsilon].
\end{aligned} \tag{13}$$

From the expectation condition and the bound on  $e_\epsilon$ , we get:

$$\mathbb{E}[e_\epsilon] \leq \frac{Q_i^*(s_i^{t_e}, a_i^{t_e}) - \mathbb{E} \left[ \sum_{t=0}^{n^0-1} \gamma^t r_i^{t_0} \right]}{\epsilon \rho} < \infty. \tag{14}$$

It follows that,

$$\begin{aligned}
&\lim_{e \rightarrow \infty} \Pr \left( \sup_{e' \geq e} \left| Q_i^*(s_i^{t_e}, a_i^{t_e}) - \sum_{t=0}^{n^{e'}-1} \gamma^t r_i^{t_{e'}} \right| \geq \epsilon \right) \\
&= \lim_{e \rightarrow \infty} \Pr \left( Q_i^*(s_i^{t_e}, a_i^{t_e}) - \sum_{t=0}^{n^e-1} \gamma^t r_i^{t_e} \geq \epsilon \right) \\
&= \lim_{e \rightarrow \infty} \Pr(e_\epsilon \geq e) = 0,
\end{aligned} \tag{15}$$

where the first equality is due to the monotonicity of  $\mathbb{E}[\sum_{t=0}^{n^e-1} \gamma^t r_i^{t_e}]$ .

Using Theorem 2, we conclude that  $Q_i^e(s_i^{t_e}, a_i^{t_e}) \rightarrow Q_i^*(s_i^{t_e}, a_i^{t_e})$  with probability one. Therefore, as  $n^e \rightarrow T$ , the cooperative phase dominates, and the Q-values converge to the optimal policy for each agent  $i$ .

## REFERENCES

- [1] C. Pelekis and J. Ramon, "Hoeffding's inequality for sums of weakly dependent random variables," 2015. [Online]. Available: <https://arxiv.org/abs/1507.06871>
- [2] A. N. Shiryaev, "Probability, volume 95 of," *Graduate texts in mathematics*, p. 81, 1996.